rules/rules_function_elim_pairwise.v
@@ -1,0 +1,414 @@
+(*
+
+  Copyright 2014 Cornell University
+  Copyright 2015 Cornell University
+  Copyright 2016 Cornell University
+  Copyright 2017 Cornell University
+  Copyright 2018 Cornell University
+
+  This file is part of VPrl (the Verified Nuprl project).
+
+  VPrl is free software: you can redistribute it and/or modify
+  it under the terms of the GNU General Public License as published by
+  the Free Software Foundation, either version 3 of the License, or
+  (at your option) any later version.
+
+  VPrl is distributed in the hope that it will be useful,
+  but WITHOUT ANY WARRANTY; without even the implied warranty of
+  MERCHANTABILITY or FITNESS FOR A PARTICULAR PURPOSE.  See the
+  GNU General Public License for more details.
+
+  You should have received a copy of the GNU General Public License
+  along with VPrl.  If not, see <http://www.gnu.org/licenses/>.
+
+
+  Websites: http://nuprl.org/html/verification/
+            http://nuprl.org/html/Nuprl2Coq
+            https://github.com/vrahli/NuprlInCoq
+
+  Authors: Abhishek Anand & Vincent Rahli
+
+*)
+
+
+Require Export rules_function_elim.
+Require Export functionality.
+
+
+
+Hint Rewrite @vars_hyps_substitute_hyps : slow.
+
+
+
+(* [17] ============ FUNCTION ELIMINATION ============ *)
+
+(**
+
+<<
+   H, f : x:A->B[x], J |- C ext e[z\axiom]
+
+     By perFunctionElimination s z
+
+     H, f : x:A->B[x], J |- a in A
+     H, f : x:A->B[x], J, z : (f a) in B[a] |- C ext e
+>>
+
+ *)
+
+Lemma rule_function_elimination_pairwise_true3 {p} :
+  forall lib (A B C a e : NTerm) ea,
+  forall f x z : NVar,
+  forall H J : @barehypotheses p,
+    pairwise_rule_true3
+      lib
+      (rule_function_elimination
+         A B C a e
+         ea
+         f x z
+         H J).
+Proof.
+  unfold rule_function_elimination, pairwise_rule_true3, wf_bseq, closed_type_baresequent, closed_extract_baresequent; simpl.
+  intros; repnd.
+  clear cargs.
+
+  (* We prove the well-formedness of things *)
+  destseq; allsimpl.
+  dLin_hyp; exrepnd.
+  rename Hyp into hyp1.
+  rename Hyp0 into hyp2.
+  destruct hyp1 as [ ws1 hyp1 ].
+  destruct hyp2 as [ ws2 hyp2 ].
+  destseq; allsimpl; proof_irr; GC.
+
+  assert (wf_csequent (snoc H (mk_hyp f (mk_function A x B)) ++ J)
+                      ||- (mk_concl C (subst e z mk_axiom))) as wfc.
+  {
+    clear hyp1 hyp2.
+    unfold wf_csequent, closed_type, closed_extract, wf_sequent, wf_concl; simpl.
+    prove_seq; eauto 3 with slow.
+    apply covered_subst; eauto 2 with slow.
+    eapply covered_subvars;[|eauto].
+    autorewrite with slow; simpl.
+    rw subvars_eq; introv i; simpl.
+    repeat (allrw @in_snoc; allrw @in_app_iff).
+    repndors; tcsp.
+  }
+  exists wfc.
+  unfold wf_csequent, wf_sequent, wf_concl in wfc; allsimpl; repnd; proof_irr; GC.
+
+  (* We prove some simple facts on our sequents *)
+  assert (disjoint (free_vars A) (vars_hyps J)
+          # disjoint (remove_nvars [x] (free_vars B)) (vars_hyps J)
+          # subvars (free_vars a) (snoc (vars_hyps H) f ++ vars_hyps J)
+          # wf_term a
+          # !LIn z (free_vars C)
+          # !LIn z (vars_hyps H)
+          # !LIn z (vars_hyps J)
+          # (z <> f)
+          # !LIn f (vars_hyps H)
+          # !LIn f (vars_hyps J)
+          # !LIn f (free_vars A)
+          # (x <> f -> !LIn f (free_vars B))) as vhyps.
+  {
+    clear hyp1 hyp2.
+    dwfseq.
+    sp;
+      try (complete (introv i; discover; allunfold @disjoint; discover; auto));
+      try (complete (assert (LIn f (remove_nvars [x] (free_vars B)))
+                      by (rw in_remove_nvars; rw in_single_iff; sp);
+                     discover; auto));
+      try (complete (apply wf_member_iff in wfct0; sp));
+      try (complete (generalize (wfh10 z); rw in_app_iff; rw in_snoc; sp));
+      try (complete (generalize (wfh10 f); rw in_remove_nvars; simpl; intro i;
+                     dest_imp i hyp));
+      try complete (pose proof (wfc1 z) as xx; autodimp xx hyp;
+                    rw in_app_iff in xx; rw in_snoc in xx; repndors; tcsp).
+  }
+
+  destruct vhyps as [ daj vhyps ].
+  destruct vhyps as [ dbj vhyps ].
+  destruct vhyps as [ sva vhyps ].
+  destruct vhyps as [ wa vhyps ].
+  destruct vhyps as [ nizc vhyps ].
+  destruct vhyps as [ nizh vhyps ].
+  destruct vhyps as [ nizj vhyps ].
+  destruct vhyps as [ nzf vhyps ].
+  destruct vhyps as [ nifh vhyps ].
+  destruct vhyps as [ nifj vhyps ].
+  destruct vhyps as [ nifa nifb ].
+  (* done with proving these simple facts *)
+
+  seq_true_pairwise.
+
+  duplicate sim as simapp.
+
+  rw @similarity_app in sim; simpl in sim; exrepnd; subst; cpx.
+  rw @similarity_snoc in sim5; simpl in sim5; exrepnd; subst; cpx.
+  lsubst_tac.
+  rw @equality_in_function in sim2; repnd.
+
+  seq_true_pairwise in hyp2.
+  pose proof (hyp2 (snoc (snoc s1a0 (f, t1) ++ s1b) (z, mkc_axiom))
+                   (snoc (snoc s2a0 (f, t2) ++ s2b) (z, mkc_axiom))) as hyp2.
+  repeat (autodimp hyp2 h); exrepnd.
+
+  {
+    (* similarity *)
+
+    assert (wf_term (mk_member (mk_apply (mk_var f) a) (subst B x a))) as wm.
+    {
+      apply wf_member; sp; try (apply wf_apply; sp).
+      apply subst_preserves_wf_term; sp.
+    }
+
+    assert (cover_vars (mk_member (mk_apply (mk_var f) a) (subst B x a))
+                       (snoc s1a0 (f, t1) ++ s1b)) as cm.
+    {
+      apply cover_vars_member; sp.
+      apply cover_vars_apply; sp.
+      apply cover_vars_var.
+      rw @dom_csub_app; rw @dom_csub_snoc; rw in_app_iff; rw in_snoc; simpl; sp.
+      rw @cover_vars_eq; rw @dom_csub_app; rw @dom_csub_snoc; insub.
+      (* begin proof of last cover_vars *)
+      rw @cover_vars_eq; rw @cover_vars_covered; apply covered_subst; sp.
+      rw @dom_csub_app; rw @dom_csub_snoc; simpl.
+      rw cons_app; apply covered_app_weak_l.
+      clear sim2 sim5; unfold cover_vars_upto in c2; unfold covered.
+      prove_subvars c2; allsimpl; sp.
+      rw @dom_csub_csub_filter in l; rw in_remove_nvars in l; rw in_single_iff in l.
+      rw in_snoc; sp.
+      clear hyp1; rw @covered_equality in ct0; repnd.
+      unfold covered; unfold covered in ct1.
+      rw @vars_hyps_app in ct1; rw @vars_hyps_snoc in ct1; simpl in ct1.
+      rw @dom_csub_app; rw @dom_csub_snoc; simpl.
+      allapply @similarity_dom; repnd; allrw; rw @vars_hyps_substitute_hyps; sp.
+      (* end proof of last cover_vars *)
+    }
+
+    sim_snoc.
+    dands; auto.
+    lsubst_tac.
+    rw @member_eq.
+    rw <- @member_member_iff.
+
+    seq_true_pairwise in hyp1.
+    generalize (hyp1 (snoc s1a0 (f, t1) ++ s1b)
+                     (snoc s2a0 (f, t2) ++ s2b));
+      clear hyp1; intros hyp1.
+    repeat (autodimp hyp1 h); exrepnd.
+    lsubst_tac.
+    allapply @member_if_inhabited.
+    rw @tequality_mkc_member in hyp0; repnd.
+    unfold member in hyp1.
+    apply sim2 in hyp1.
+
+    assert (disjoint (remove_nvars [x] (free_vars B)) (dom_csub s1b)) as disj1.
+    {
+      apply similarity_dom in sim1; repnd.
+      rw sim7.
+      rewrite vars_hyps_substitute_hyps; auto.
+    }
+
+    apply equality_refl in hyp1.
+    unfold member in *.
+    repeat (lsubstc_subst_aeq2;[]).
+    repeat (substc_lsubstc_vars3;[]).
+    repeat (lsubstc_weak;[]).
+    proof_irr.
+    auto.
+  }
+
+  {
+    (* eq_hyps *)
+
+    prove_eq_hyps_snoc.
+
+    { apply wf_member; eauto 2 with slow.
+      eapply wf_apply; eauto 2 with slow. }
+
+    { apply cover_vars_member; dands; eauto 2 with slow.
+      { apply cover_vars_apply; dands; eauto 2 with slow.
+        { apply cover_vars_var; rw @dom_csub_app; rw @dom_csub_snoc; simpl.
+          rw in_app_iff; rw @in_snoc; tcsp. }
+        { apply cover_vars_eq.
+          rw @dom_csub_app; rw @dom_csub_snoc; simpl.
+          apply similarity_dom in sim6; repnd.
+          apply similarity_dom in sim1; repnd.
+          autorewrite with slow in *.
+          allrw; auto. } }
+      { apply cover_vars_lsubst_if; simpl.
+        { eapply subvars_trans;[exact c2|]; simpl.
+          rw @dom_csub_app; rw @dom_csub_snoc; simpl.
+          apply subvars_cons_lr.
+          rw @dom_csub_csub_filter.
+          apply subvars_remove_nvars.
+          repeat apply subvars_app_weak_l.
+          apply subvars_snoc_weak; auto. }
+        { introv h; repndors; tcsp; ginv.
+          apply cover_vars_eq.
+          rw @dom_csub_app; rw @dom_csub_snoc; simpl.
+          apply similarity_dom in sim6; repnd.
+          apply similarity_dom in sim1; repnd.
+          autorewrite with slow in *.
+          allrw; auto. } } }
+
+    { apply cover_vars_member; dands; eauto 2 with slow.
+      { apply cover_vars_apply; dands; eauto 2 with slow.
+        { apply cover_vars_var; rw @dom_csub_app; rw @dom_csub_snoc; simpl.
+          rw in_app_iff; rw @in_snoc; tcsp. }
+        { apply cover_vars_eq.
+          rw @dom_csub_app; rw @dom_csub_snoc; simpl.
+          apply similarity_dom in sim6; repnd.
+          apply similarity_dom in sim1; repnd.
+          autorewrite with slow in *.
+          allrw; auto. } }
+      { apply cover_vars_lsubst_if; simpl.
+        { eapply subvars_trans;[exact c2|]; simpl.
+          rw @dom_csub_app; rw @dom_csub_snoc; simpl.
+          apply subvars_cons_lr.
+          rw @dom_csub_csub_filter.
+          apply subvars_remove_nvars.
+          repeat apply subvars_app_weak_l.
+          apply subvars_snoc_weak; auto.
+          apply similarity_dom in sim6; repnd; allrw; auto. }
+        { introv h; repndors; tcsp; ginv.
+          apply cover_vars_eq.
+          rw @dom_csub_app; rw @dom_csub_snoc; simpl.
+          apply similarity_dom in sim6; repnd.
+          apply similarity_dom in sim1; repnd.
+          autorewrite with slow in *.
+          allrw; auto. } } }
+
+    lsubst_tac.
+    apply tequality_mkc_member_if_equal.
+
+    seq_true_pairwise in hyp1.
+    pose proof (hyp1 (snoc s1a0 (f,t1) ++ s1b) (snoc s2a0 (f,t2) ++ s2b)) as hyp1.
+    repeat (autodimp hyp1 h); exrepnd;[].
+    lsubst_tac.
+
+    allapply @member_if_inhabited.
+    rw @tequality_mkc_member in hyp0; repnd.
+    autodimp hyp0 hyp.
+    applydup hyp3 in hyp1; clear hyp3.
+    rename hyp0 into eqa.
+
+    applydup sim5 in eqa.
+
+    dup eqh as eqhapp.
+    rw @eq_hyps_app in eqh; simpl in eqh; exrepnd; subst; cpx.
+    apply app_split in eqh0; repnd; allrw length_snoc;
+      try (complete (allrw; sp)); subst; cpx.
+    apply app_split in eqh2; repnd; allrw length_snoc;
+      try (complete (allrw; sp)); subst; cpx.
+
+    rw @eq_hyps_snoc in eqh5; simpl in eqh5; exrepnd; subst; cpx.
+    lsubst_tac.
+    rw @tequality_function in eqh0; repnd.
+
+    applydup eqh0 in eqa as teq.
+
+    assert (disjoint (remove_nvars [x] (free_vars B)) (dom_csub s1b0)) as disj1.
+    {
+      apply similarity_dom in sim1; repnd.
+      rw sim7.
+      rewrite vars_hyps_substitute_hyps; auto.
+    }
+
+    assert (disjoint (remove_nvars [x] (free_vars B)) (dom_csub s2b0)) as disj2.
+    {
+      apply sub_eq_hyps_dom in eqh1; repnd.
+      rw eqh1; auto.
+    }
+
+    repeat (substc_lsubstc_vars3;[]).
+
+    applydup sim2 in eqa as eqf.
+
+    assert (tequality lib (lsubstc (subst B x a) wT (snoc s1a (f, t0) ++ s1b0) cT)
+                      (lsubstc (subst B x a) wT (snoc s2a (f, t3) ++ s2b0) cT0)).
+    { repeat (lsubstc_subst_aeq2;[]).
+      repeat (substc_lsubstc_vars3;[]).
+      repeat (lsubstc_weak;[]).
+      proof_irr.
+      exact teq.
+    }
+
+    assert (tequality
+              lib
+              (lsubstc (subst B x a) wT (snoc s1a (f, t0) ++ s1b0) cT)
+              (lsubstc_vars B w2 (csub_filter s1a [x]) [x] c2)
+              [[x \\ lsubstc a wa (snoc s1a (f, t0) ++ s1b0) c3]]).
+    repeat (lsubstc_subst_aeq2;[]).
+    repeat (substc_lsubstc_vars3;[]).
+    repeat (lsubstc_weak;[]).
+    proof_irr.
+    unfold equality in eqf; exrepnd; eapply tequality_if_nuprl; eauto.
+    dands; auto.
+    repeat (lsubstc_subst_aeq2;[]).
+    repeat (substc_lsubstc_vars3;[]).
+    repeat (lsubstc_weak;[]).
+    proof_irr; auto.
+  }
+
+  (* conclusion *)
+
+  lsubst_tac; sp.
+
+  assert (wf_term (@mk_axiom p)) as wfax by eauto 2 with slow.
+
+  repeat (lsubstc_subst_aeq2;[]).
+  allrw @lsubstc_mk_axiom.
+  repeat (substc_lsubstc_vars3;[]).
+  proof_irr.
+
+  pose proof (lsubstc_snoc_move
+                e
+                (snoc s1a0 (f, t1) ++ s1b)
+                []
+                z
+                mkc_axiom
+                wfce) as xx1.
+  allrw app_nil_r.
+  allrw @dom_csub_app.
+  allrw @dom_csub_snoc.
+  allsimpl.
+  pose proof (xx1 pt0) as xx2; clear xx1.
+  autodimp xx2 hyp.
+  { apply similarity_dom in sim6; repnd.
+    rewrite sim7.
+    apply similarity_dom in sim1; repnd.
+    rewrite sim8.
+    rewrite vars_hyps_substitute_hyps; auto.
+    rw in_app_iff; rw in_snoc; intro i; repndors; tcsp.
+  }
+  exrepnd.
+  proof_irr.
+  rewrite <- xx0; clear xx0.
+
+  pose proof (lsubstc_snoc_move
+                e
+                (snoc s2a0 (f, t2) ++ s2b)
+                []
+                z
+                mkc_axiom
+                wfce) as xx1.
+  allrw app_nil_r.
+  allrw @dom_csub_app.
+  allrw @dom_csub_snoc.
+  allsimpl.
+  pose proof (xx1 pt3) as xx2; clear xx1.
+  autodimp xx2 hyp.
+  { apply similarity_dom in sim6; repnd.
+    rewrite sim6.
+    apply similarity_dom in sim1; repnd.
+    rewrite sim1.
+    rewrite vars_hyps_substitute_hyps; auto.
+    rw in_app_iff; rw in_snoc; intro i; repndors; tcsp.
+  }
+  exrepnd.
+  proof_irr.
+  rewrite <- xx0; clear xx0.
+
+  auto.
+Qed.
